Verifying Frames2

src/SDK/Serialize/Frames2.dfy
@@ -50,12 +50,12 @@ module Frames2 {
     iv: seq<uint8>,
     encContent: seq<uint8>,
     authTag: seq<uint8>)
-  // | NonFramed(
-  //   header: Header.Header,
-  //   iv: seq<uint8>,
-  //   encContent: seq<uint8>,
-  //   authTag: seq<uint8>
-  // )
+  | NonFramed(
+    header: Header.Header,
+    iv: seq<uint8>,
+    encContent: seq<uint8>,
+    authTag: seq<uint8>
+  )
 
   predicate IvTagLengths(frame: Frame){
     && |frame.iv| == frame.header.suite.encrypt.ivLength as nat
@@ -79,13 +79,13 @@ module Frames2 {
     && |frame.encContent| <= frame.header.body.frameLength as nat
   witness *
 
-  // type NonFramed = frame: Frame
-  // |
-  //   && frame.NonFramed?
-  //   && IvTagLengths(frame)
-  //   && frame.header.body.contentType.NonFramed?
-  //   && |frame.encContent| < SAFE_MAX_ENCRYPT
-  // witness *
+  type NonFramed = frame: Frame
+  |
+    && frame.NonFramed?
+    && IvTagLengths(frame)
+    && frame.header.body.contentType.NonFramed?
+    && |frame.encContent| < SAFE_MAX_ENCRYPT
+  witness *
   
   const SAFE_MAX_ENCRYPT := 0xFFFFFFFE0 // 2^36 - 32
 
@@ -97,10 +97,10 @@ module Frames2 {
       && ReadUInt32(ReadableBytes(ret, 0)).Success?
       && ReadUInt32(ReadableBytes(ret, 0)).value.thing != ENDFRAME_SEQUENCE_NUMBER
   {
-    UInt32ToSeq(regularFrame.seqNum)
-    + regularFrame.iv
-    + regularFrame.encContent
-    + regularFrame.authTag
+    WriteUint32(regularFrame.seqNum)
+    + Write(regularFrame.iv)
+    + Write(regularFrame.encContent)
+    + Write(regularFrame.authTag)
   }
 
   function method ReadRegularFrame(
@@ -108,6 +108,13 @@ module Frames2 {
     header: FramedHeader
   )
     :(res: ReadCorrect<RegularFrame>)
+    ensures res.Success?
+    ==>
+      && var Data(thing, tail) := res.value;
+      && tail.data == bytes.data
+      && |tail.data| >= tail.start >= bytes.start
+      && bytes.data[bytes.start..tail.start] == tail.data[bytes.start..tail.start]
+      && WriteRegularFrame(thing) == tail.data[bytes.start..tail.start]
     ensures CorrectlyRead(bytes, res, WriteRegularFrame)
   {
 
@@ -129,103 +136,98 @@ module Frames2 {
     Success(Data(regularFrame, authTag.tail))
   }
 
-  // function method WriteFinalFrame(
-  //   finalFrame: FinalFrame
-  // )
-  //   :(ret: seq<uint8>)
-  //   ensures 
-  //     && ReadUInt32(ReadableBytes(ret, 0)).Success?
-  //     && ReadUInt32(ReadableBytes(ret, 0)).value.thing == ENDFRAME_SEQUENCE_NUMBER
-  // {
-  //   UInt32ToSeq(ENDFRAME_SEQUENCE_NUMBER)
-  //   + UInt32ToSeq(finalFrame.seqNum)
-  //   + Write(finalFrame.iv)
-  //   + UInt32ToSeq(|finalFrame.encContent| as uint32)
-  //   + Write(finalFrame.encContent)
-  //   + Write(finalFrame.authTag)
-  // }
+  function method WriteFinalFrame(
+    finalFrame: FinalFrame
+  )
+    :(ret: seq<uint8>)
+    ensures 
+      && ReadUInt32(ReadableBytes(ret, 0)).Success?
+      && ReadUInt32(ReadableBytes(ret, 0)).value.thing == ENDFRAME_SEQUENCE_NUMBER
+  {
+    WriteUint32(ENDFRAME_SEQUENCE_NUMBER)
+    + WriteUint32(finalFrame.seqNum)
+    + Write(finalFrame.iv)
+    + WriteUint32Seq(finalFrame.encContent)
+    + Write(finalFrame.authTag)
+  }
 
-  // function method ReadFinalFrame(
-  //   bytes: ReadableBytes,
-  //   header: FramedHeader
-  // )
-  //   :(res: ReadCorrect<FinalFrame>)
-  //   ensures
-  //     res.Success?
-  //   ==>
-  //     && var Data(thing, tail) := res.value;
-  //     && tail.data == bytes.data
-  //     && tail.Tail?
-  //     && tail.start == bytes.pos
-  //     && |tail.data| >= tail.pos >= bytes.pos
-  //     && WriteFinalFrame(thing) == tail.data[tail.start..tail.pos]
-  //   // ensures CorrectlyRead(bytes, res, WriteFinalFrame)
-  // {
-  //   var finalFrameSignal :- ReadUInt32(bytes);
-  //   :- Need(finalFrameSignal.thing == ENDFRAME_SEQUENCE_NUMBER, Error("bad"));
+  function method ReadFinalFrame(
+    bytes: ReadableBytes,
+    header: FramedHeader
+  )
+    :(res: ReadCorrect<FinalFrame>)
+    ensures res.Success?
+    ==>
+      && var Data(thing, tail) := res.value;
+      && tail.data == bytes.data
+      && |tail.data| >= tail.start >= bytes.start
+      && bytes.data[bytes.start..tail.start] == tail.data[bytes.start..tail.start]
+      && WriteFinalFrame(thing) == tail.data[bytes.start..tail.start]
+    ensures CorrectlyRead(bytes, res, WriteFinalFrame)
+  {
+    var finalFrameSignal :- ReadUInt32(bytes);
+    :- Need(finalFrameSignal.thing == ENDFRAME_SEQUENCE_NUMBER, Error("bad"));
 
-  //   var sequenceNumber :- ReadUInt32(finalFrameSignal.tail);
-  //   var iv :- Read(sequenceNumber.tail, header.suite.encrypt.ivLength as nat);
-  //   var contentLength :- ReadUInt32(iv.tail);
-  //   :- Need(contentLength.thing <= header.body.frameLength, Error("bad"));
-  //   var encContent :- Read(contentLength.tail, contentLength.thing as nat);
-  //   var authTag :- Read(encContent.tail, header.suite.encrypt.tagLength as nat);
+    var sequenceNumber :- ReadUInt32(finalFrameSignal.tail);
+    var iv :- Read(sequenceNumber.tail, header.suite.encrypt.ivLength as nat);
+    var encContent :- ReadUint32Seq(iv.tail);
+    :- Need(|encContent.thing| as uint32 <= header.body.frameLength, Error("bad"));
+    var authTag :- Read(encContent.tail, header.suite.encrypt.tagLength as nat);
 
-  //   var finalFrame: FinalFrame := Frame.FinalFrame(
-  //     header,
-  //     sequenceNumber.thing,
-  //     iv.thing,
-  //     encContent.thing,
-  //     authTag.thing
-  //   );
+    var finalFrame: FinalFrame := Frame.FinalFrame(
+      header,
+      sequenceNumber.thing,
+      iv.thing,
+      encContent.thing,
+      authTag.thing
+    );
 
-  //   Success(Data(finalFrame, authTag.tail.(start := bytes.pos)))
-  // }
+    Success(Data(finalFrame, authTag.tail))
+  }
 
-  // function method ReadNonFrame(
-  //   bytes: ReadableBytes,
-  //   header: NonFramedHeader
-  // )
-  //   :(res: ReadCorrect<NonFramed>)
-  //   ensures
-  //     res.Success?
-  //   ==>
-  //     && var Data(thing, tail) := res.value;
-  //     && tail.data == bytes.data
-  //     && tail.Tail?
-  //     && tail.start == bytes.pos
-  //     && |tail.data| >= tail.pos >= bytes.pos
-  //     && WriteNonFramed(thing) == tail.data[tail.start..tail.pos]
-  //   // ensures CorrectlyRead(bytes, res, WriteNonFramed)
-  // {
-  //   var iv :- Read(bytes, header.suite.encrypt.ivLength as nat);
-  //   var contentLength :- ReadUInt64(iv.tail);
-  //   :- Need(contentLength.thing as nat < SAFE_MAX_ENCRYPT, Error("Too Much"));
-  //   var encContent :- Read(contentLength.tail, contentLength.thing as nat);
-  //   var authTag :- Read(encContent.tail, header.suite.encrypt.tagLength as nat);
+  function method ReadNonFrame(
+    bytes: ReadableBytes,
+    header: NonFramedHeader
+  )
+    :(res: ReadCorrect<NonFramed>)
+    ensures res.Success?
+    ==>
+      && var Data(thing, tail) := res.value;
+      && tail.data == bytes.data
+      && |tail.data| >= tail.start >= bytes.start
+      && bytes.data[bytes.start..tail.start] == tail.data[bytes.start..tail.start]
+      && WriteNonFramed(thing) == tail.data[bytes.start..tail.start]
+    ensures CorrectlyRead(bytes, res, WriteNonFramed)
+  {
+    var iv :- Read(bytes, header.suite.encrypt.ivLength as nat);
+    // Checking only the content length _before_ reading it into memory
+    // is just a nice thing to do given the sizes involved.
+    var contentLength :- ReadUInt64(iv.tail);
+    :- Need(contentLength.thing as nat < SAFE_MAX_ENCRYPT, Error("Too Much"));
+    var encContent :- ReadUint64Seq(iv.tail);
+    var authTag :- Read(encContent.tail, header.suite.encrypt.tagLength as nat);
 
-  //   var nonFramed: NonFramed := Frame.NonFramed(
-  //     header,
-  //     iv.thing,
-  //     encContent.thing,
-  //     authTag.thing
-  //   );
+    var nonFramed: NonFramed := Frame.NonFramed(
+      header,
+      iv.thing,
+      encContent.thing,
+      authTag.thing
+    );
 
-  //   Success(Data(nonFramed, authTag.tail.(start := bytes.pos)))
-  // }
+    Success(Data(nonFramed, authTag.tail))
+  }
 
-  // // The Encryption SDK no longer supports writing Non-Framed Data.
-  // // That is why this is a function and not a function method.
-  // // This is here to support correct reading of Non-Framed Data.
-  // function WriteNonFramed(
-  //   nonFramed: NonFramed
-  // )
-  //   :(ret: seq<uint8>)
-  // {
-  //   Write(nonFramed.iv)
-  //   + UInt64ToSeq(|nonFramed.encContent| as uint64)
-  //   + Write(nonFramed.encContent)
-  //   + Write(nonFramed.authTag)
-  // }
+  // The Encryption SDK no longer supports writing Non-Framed Data.
+  // That is why this is a function and not a function method.
+  // This is here to support correct reading of Non-Framed Data.
+  function WriteNonFramed(
+    nonFramed: NonFramed
+  )
+    :(ret: seq<uint8>)
+  {
+    Write(nonFramed.iv)
+    + WriteUint64Seq(nonFramed.encContent)
+    + Write(nonFramed.authTag)
+  }
 
 }
